Added a second proof of teleportation that uses a bell measurement proof

src/Gates/GateDefinitions.v
@@ -1,4 +1,7 @@
 Require Import ZXCore.
+Require Import CoreRules.
+Require Import GateRules.
+Require Setoid.
 From VyZX Require Import Proportional.
 
 Local Open Scope ZX_scope.
@@ -29,5 +32,97 @@ Notation "'_NOTC_R'" :=
 
 Notation "'_3_CNOT_SWAP_'" :=
   (_CNOT_ ⟷ _NOTC_ ⟷ _CNOT_).
-  
 
+Definition bell_state_prep :=
+  (((X 0 1 0) ↕ (X 0 1 0)) ⟷ (□ ↕ —) ⟷ 
+  ((Z 1 2 0 ↕ —) ⟷ (— ↕ X 2 1 0))).
+
+Definition bell_measurement (a b : nat) :=
+  (_CNOT_ ⟷ (((Z 1 0 ((INR a) * PI))) ↕ (X 1 0 ((INR b) * PI)))).
+
+Lemma bell_measurement_eq : forall a b,
+  bell_measurement a b ∝= (Z 1 1 (INR a * PI) ⟷ X 1 1 (INR b * PI)) ↕ — ⟷ ⊃.
+Proof.
+  intros; unfold bell_measurement.
+  unfold bell_measurement.
+  rewrite compose_assoc.
+  rewrite <- (stack_compose_distr Wire (Z 1 0 _) (X 2 1 0)).
+  rewrite X_spider_1_1_fusion.
+  rewrite wire_removal_l.
+  rewrite Rplus_0_l.
+  assert (H : ((Z 1 0 (INR a * PI) ↕ X 2 0 (INR b * PI))) ∝=
+  (((Z 1 0 (INR a * PI) ↕ — ↕ —) ⟷ (X 2 0 (INR b * PI))))).
+  { rewrite stack_assoc.      
+    simpl_casts.
+    rewrite <- (stack_empty_l (X 2 0 _)) at 2.
+    rewrite <- (stack_compose_distr (Z 1 0 _) ⦰ (— ↕ —) (X 2 0 _)).
+    bundle_wires.
+    cleanup_zx.
+    reflexivity. }
+  rewrite H.
+  rewrite <- compose_assoc.
+  rewrite <- stack_compose_distr.
+  assert (H0 : — ∝= n_wire 1).
+  {
+    bundle_wires.
+    reflexivity.
+  }
+  rewrite H0.
+  rewrite (dominated_Z_spider_fusion_top_left 0 0).
+  simpl.
+  cleanup_zx.
+  replace (INR b * PI)%R with (INR b * PI + 0)%R by lra.
+  rewrite <- (dominated_X_spider_fusion_top_right 1 0 1 0).
+  rewrite <- cup_X.
+  rewrite 2 Rplus_0_r.
+  rewrite <- compose_assoc.
+  rewrite <- (stack_compose_distr (Z 1 1 _) (X 1 1 _) (n_wire 1) (n_wire 1)).
+  cleanup_zx.
+  reflexivity.
+  Unshelve.
+  all:lia. Qed.
+
+Definition teleportation_2 
+  (a b : nat) :=
+  (— ↕ bell_state_prep) ⟷ ((bell_measurement a b) ↕ 
+                          (X 1 1 (INR b * PI) ⟷ (Z 1 1 (INR a * PI)))).
+
+Lemma teleportation_2_correct : forall a b, teleportation_2 a b ∝= —.
+Proof.
+  intros; unfold teleportation_2.
+  rewrite bell_measurement_eq.
+  rewrite bell_state_prep_correct.
+  rewrite <- (wire_removal_l (X 1 1 _ ⟷ Z 1 1 _)).
+  rewrite stack_compose_distr.
+  rewrite stack_assoc.
+  simpl_casts.
+  rewrite <- compose_assoc.
+  rewrite <- (stack_compose_distr — (Z 1 1 _ ⟷ X 1 1 _) ⊂ (— ↕ —)).
+  rewrite wire_removal_l.
+  bundle_wires.
+  cleanup_zx.
+  rewrite <- (wire_removal_r (Z 1 1 _ ⟷ X 1 1 _)).
+  rewrite <- compose_empty_l.
+  rewrite stack_compose_distr.
+  rewrite <- (wire_removal_l (X 1 1 _ ⟷ Z 1 1 _)).
+  rewrite <- (compose_empty_r ⊃).
+  rewrite stack_compose_distr.
+  repeat rewrite compose_assoc.
+  rewrite <- (compose_assoc (— ↕ ⊂)).
+  rewrite yank_l.
+  cleanup_zx.
+  simpl_casts.
+  repeat rewrite compose_assoc.
+  rewrite <- (compose_assoc (X 1 1 _) (X 1 1 _) (Z 1 1 _)).
+  rewrite X_spider_1_1_fusion.
+  replace (INR b * PI + INR b * PI)%R with (INR b * 2 * PI)%R by lra.
+  rewrite X_2_PI.
+  cleanup_zx.
+  rewrite Z_spider_1_1_fusion.
+  replace (INR a * PI + INR a * PI)%R with (INR a * 2 * PI)%R by lra.
+  rewrite Z_2_PI.
+  cleanup_zx.
+  reflexivity. 
+  Unshelve.
+  all: lia.
+  Qed.
